> [!definition]
> ---
> Definition of exponentiation with positive integer exponents
> - If $a$ is any number and $n$ is a positive integer then,
> $$a^n = \underbrace{a \cdot a \cdot a \cdot \cdot \cdot a}_{n \textrm{ times}}$$
> 

**Example**
$$3^5=3\cdot3\cdot3\cdot3\cdot3=243$$
### Negative Integers
Consider
$$(-2)^4 \qquad \textrm{ and } \qquad -2^4$$
These cases will have different values once evaluated.
$$(-2)^4 = (-2)(-2)(-2)(-2)=16$$
$$-2^4=-(2^4)=-(2\cdot2\cdot2\cdot2)=-(16)=-16$$
### Zero Exponents
> [!info]
> ---
> **Zero Exponents Case**
> - $a$ should not be 0
> - $0^0$ is not defined
> $$a^0=1 \textrm{\qquad provided } \qquad a \neq 0$$

### Properties of Exponents
| Property                                                                                                    | Example                                                                                                                    |
| ----------------------------------------------------------------------------------------------------------- | -------------------------------------------------------------------------------------------------------------------------- |
| $a^n a^m = a^{n+m}$                                                                                         | $a^{-9} a^4 = a^{-9+4} = a^{-5}$                                                                                           |
| $(a^n)^m = a^{nm}$                                                                                          | (a^7)^3 = a^{(7)(3)} = a^{21}                                                                                              |
| $\frac{a^n}{a^m} = \left\{\begin{align}a^{n-m} \\\frac{1}{a^{m-n}}\end{align}\right. \quad, \quad a \neq 0$ | $\begin{align}\frac{a^4}{a^{11}}=a^{4-11}=a^{-7}\\ \frac{a^4}{a^{11}}=\frac{1}{a^{11-4}}=\frac{1}{a^7}=a^{-7} \end{align}$ |
| $(ab)^n = a^nb^n$                                                                                           | $(ab)^{-4}=a^{-4}b^{-4}$                                                                                                   |
| $(\frac{a}{b})^n = \frac{a^n}{b^n}, \quad b \neq 0$                                                         | $(\frac{a}{b})^8 = \frac{a^8}{b^8}$                                                                                        |
| $(\frac{a}{b})^{-n} = (\frac{b}{a})^n = \frac{b^n}{a^n}$                                                    | $(\frac{a}{b})^{-10} = (\frac{b}{a})^{10} = \frac{b^{10}}{a^{10}}$                                                         |
| $(ab)^{-n} = \frac{1}{(ab)^n}$                                                                              | $(ab)^{-20} = \frac{1}{(ab)^{20}}$                                                                                         |
| $\frac{1}{a^{-n}=a^n}$                                                                                      | $\frac{a^{-2}} = a^2$                                                                                                      |
| $\frac{a^{-n}}{b^{-m}} = \frac{b^m}{a^n}$                                                                   | $\frac{a^{-6}}{b^{-17}} = \frac{b^{17}}{a^6}$                                                                              |
| $(a^nb^m)^k = a^{nk}b^{mk}$                                                                                 | $(a^4b^{-9})^3 = a^{(4)(3)}b^{(-9)(3)} = a^{12}b^{-27}$                                                                    |
| $(\frac{a^n}{b^m})^k = \frac{a^{nk}}{b^{mk}}$                                                               | $(\frac{a^6}{b^5})^2 = \frac{a^{(6)(2)}}{b^{(5)(2)}} = \frac{a^{12}}{b^{10}}$                                                                                                                           |

> [!tip]
> ---
> Properties can be extended out to as many terms or factors as needed. For example, property 4 can be extended as follows.
> $$(abcd)^n = a^nb^nc^nd^n$$

#### Common Mistakes
$(ab)^{-2} = \frac{1}{(ab)^2}$
Correct: $\qquad ab^{-2} = a\frac{1}{b^2} = \frac{a}{b^2}$
Incorrect: $\qquad ab^{-2} \neq \frac{1}{ab^2}$

$\frac{1}{(3a)^{-5}} = (3a)^5$
Correct: $\qquad \frac{1}{3a^{-5}} = \frac{1}{3}\frac{1}{a^{-5}} = \frac{1}{3}a^5$
Incorrect: $\qquad \frac{1}{3a^{-5}} \neq 3a^5$

### Assignment
**Problem**
1. $(4x^{-4}y^5)^3$
2. $(-10z^2y^{-4})^2(z^3y)^{-5}$
3. $\frac{n^{-2}m}{7m^{-4}n^{-3}}$
4. $\frac{5x^{-1}y^{-4}}{(3y^5)^{-2}x^9}$
5. $(\frac{z^{-5}}{z^{-2}x^{-1}})^6$
6. $(\frac{24a^3b^{-8}}{6a^{-5}b})^{-2}$

**Solution**
1. $(4x^{-4}y^5)^3$
$$(4x^{-4}y^5)^3 = 4^3x^{-12}y^{15}$$
$$64(\frac{1}{x^{12}}y^{15}) = \frac{64y^{15}}{x^{12}}$$

2. $(-10z^2y^{-4})^2(z^3y)^{-5}$
$$(-10z^2y^{-4})^2(z^3y)^{-5} = (-10)^2z^4y^{-8}z^{-15}y^{-5}$$
$$100z^{-11}y^{-13} = \frac{100}{z^{11}y^{13}}$$

3. $\frac{n^{-2}m}{7m^{-4}n^{-3}}$
$$\frac{n^{-2}m}{7m^{-4}n^{-3}} = \frac{m^4n^3m}{7n^2} = \frac{m^5n}{7}$$

4. $\frac{5x^{-1}y^{-4}}{(3y^5)^{-2}x^9}$
$$\frac{5x^{-1}y^{-4}}{(3y^5)^{-2}x^9} = \frac{5(3y^5)^2}{xy^4x^9} = \frac{5(9)y^{10}}{xy^4x^9} = \frac{45y^6}{x^{10}}$$

5. $(\frac{z^{-5}}{z^{-2}x^{-1}})^6$
$$(\frac{z^{-5}}{z^{-2}x^{-1}}^6) = (\frac{z^2x^1}{z^5})^6 = (\frac{x}{z^3})^6 = \frac{x^6}{z^{18}}$$

6. $(\frac{24a^3b^{-8}}{6a^{-5}b})^{-2}$
$$(\frac{24a^3b^{-8}}{6a^{-5}b})^{-2} = (\frac{4a^3a^5}{b^8b})^{-2} = (\frac{4a^8}{b^9})^{-2}$$
$$(\frac{b^9}{4a^8})^2 = \frac{b^{18}}{16a^{16}}$$